\begin{proof}
    $\models (p\rightarrow q) \Rightarrow p\models q$的证明：
    \begin{align*}
        \models&\; p\rightarrow q  &\text{1}\\
        p\models&\; p &\text{2}\\
        p\models&\; q &\text{MP(1,2) 3}\\
    \end{align*}

    $p\models q \Rightarrow\; \models (p\rightarrow q) $的证明：
    \begin{align*}
        p\models&\; q &\text{1}\\
        p\models&\; p \rightarrow q &\text{变形(1) 2}\\
        \neg p\models&\; p \rightarrow q &\text{3}\\
        \models&\; p \rightarrow q &\text{由(2,3) 4}
    \end{align*}
\end{proof}